split old and new definitions in typing.typing

theories/typing/typing.v
@@ -6,32 +6,10 @@ From lrust.typing Require Import perm lft_contexts type_context cont_context.
 From lrust.lang Require Import proofmode.
 From lrust.lifetime Require Import frac_borrow reborrow borrow creation.
 
-(* TODO: Split this file into instructions.v and body.v. *)
+(* TODO: This is all still using the outdated type system. *)
 
 Section typing.
   Context `{typeG Σ}.
-
-  Definition typed_body (E : elctx) (L : llctx) (C : cctx) (T : tctx)
-                        (e : expr) : iProp Σ :=
-    (∀ tid qE, lft_ctx -∗ elctx_interp E qE -∗ llctx_interp L 1 -∗
-               (elctx_interp E qE -∗ cctx_interp tid C) -∗ tctx_interp tid T -∗
-               WP e {{ _, cont_postcondition }})%I.
-
-  Instance typed_body_llctx_permut E :
-    Proper ((≡ₚ) ==> eq ==> eq ==> eq ==> (⊢)) (typed_body E).
-  Proof.
-    intros L1 L2 HL C ? <- T ? <- e ? <-. rewrite /typed_body. by setoid_rewrite HL.
-  Qed.
-
-  Instance typed_body_mono E L:
-    Proper (flip (cctx_incl E) ==> flip (tctx_incl E L) ==> eq ==> (⊢)) (typed_body E L).
-  Proof.
-    intros C1 C2 HC T1 T2 HT e ? <-. iIntros "H".
-    iIntros (tid qE) "#LFT HE HL HC HT".
-    iMod (HT with "LFT HE HL HT") as "(HE & HL & HT)".
-    iApply ("H" with "LFT HE HL [HC] HT").
-    iIntros "HE". by iApply (HC with "LFT HC").
-  Qed.
 
   (* TODO : good notations for [typed_step] and [typed_step_ty] ? *)
   Definition typed_step (ρ : perm) e (θ : val → perm) :=
