theories/typing/programs.v
@@ -1,0 +1,34 @@
+From iris.program_logic Require Import hoare.
+From iris.base_logic Require Import big_op.
+From lrust.lang Require Export notation memcpy.
+From lrust.typing Require Export type.
+From lrust.typing Require Import perm lft_contexts type_context cont_context.
+From lrust.lang Require Import proofmode.
+From lrust.lifetime Require Import frac_borrow reborrow borrow creation.
+
+Section typing.
+  Context `{typeG Σ}.
+
+  Definition typed_body (E : elctx) (L : llctx) (C : cctx) (T : tctx)
+                        (e : expr) : iProp Σ :=
+    (∀ tid qE, lft_ctx -∗ elctx_interp E qE -∗ llctx_interp L 1 -∗
+               (elctx_interp E qE -∗ cctx_interp tid C) -∗ tctx_interp tid T -∗
+               WP e {{ _, cont_postcondition }})%I.
+
+  Instance typed_body_llctx_permut E :
+    Proper ((≡ₚ) ==> eq ==> eq ==> eq ==> (⊢)) (typed_body E).
+  Proof.
+    intros L1 L2 HL C ? <- T ? <- e ? <-. rewrite /typed_body. by setoid_rewrite HL.
+  Qed.
+
+  Instance typed_body_mono E L:
+    Proper (flip (cctx_incl E) ==> flip (tctx_incl E L) ==> eq ==> (⊢)) (typed_body E L).
+  Proof.
+    intros C1 C2 HC T1 T2 HT e ? <-. iIntros "H".
+    iIntros (tid qE) "#LFT HE HL HC HT".
+    iMod (HT with "LFT HE HL HT") as "(HE & HL & HT)".
+    iApply ("H" with "LFT HE HL [HC] HT").
+    iIntros "HE". by iApply (HC with "LFT HC").
+  Qed.
+
+End typing.
